prototype/parser.mly
@@ -6,7 +6,7 @@ open Ast
 let location start_pos end_pos =
   { start_pos; end_pos }
 
-let mkexpr desc start_pos end_pos =
+let with_location desc start_pos end_pos =
   let location = location start_pos end_pos in
   { desc; location }
 
@@ -20,6 +20,7 @@ let mkexpr desc start_pos end_pos =
 %token IN
 %token LET
 %token MATCH
+%token REF
 %token WITH
 
 /* Identifiers */
@@ -30,11 +31,14 @@ let mkexpr desc start_pos end_pos =
 /* Symbols */
 
 %token ARROW
+%token BANG
 %token BAR
+%token COLONEQUALS
 %token EQUALS
 %token HASH
 %token LPAREN
 %token RPAREN
+%token SEMI
 %token SEMISEMI
 %token UNDERSCORE
 
@@ -45,42 +49,71 @@ let mkexpr desc start_pos end_pos =
 %%
 
 phrase:
-  | d = definition SEMISEMI
-      { Definition d }
-  | HASH dir = LIDENT SEMISEMI
-      { Directive dir }
+  | statement = statement SEMISEMI
+      { let desc = Statement { statement } in
+        with_location desc $startpos $endpos }
+  | HASH directive = LIDENT SEMISEMI
+      { let desc = Directive { directive } in
+        with_location desc $startpos $endpos }
+;
+
+statement:
+  | LET binding = binding params = loption(parameters) EQUALS def = sequence_expr
+      { let desc = Definition { binding; params; def } in
+        with_location desc $startpos $endpos }
+  | expr = expr
+      { let desc = Expr { expr } in
+        with_location desc $startpos $endpos }
 ;
 
 simple_expr:
   | name = LIDENT
       { let desc = Var{ name; } in
-        mkexpr desc $startpos $endpos }
-  | LPAREN expr = expr RPAREN
+        with_location desc $startpos $endpos }
+  | BANG reference = simple_expr
+      { let desc = Deref{ reference; } in
+        with_location desc $startpos $endpos }
+  | LPAREN expr = sequence_expr RPAREN
       { expr }
   | LPAREN RPAREN
       { let desc = Unit in
-        mkexpr desc $startpos $endpos }
+        with_location desc $startpos $endpos }
 ;
 
 expr:
   | expr = simple_expr
       { expr }
-  | LET binding = binding params = loption(parameters) EQUALS def = expr IN body = expr
-      { let desc = Let{ binding; params; def; body; } in
-        mkexpr desc $startpos $endpos }
-  | FUN params = parameters ARROW body = expr
-      { let desc = Abs{ params; body } in
-        mkexpr desc $startpos $endpos }
   | fn = simple_expr args = nonempty_list(simple_expr)
       { let desc = App{ fn; args } in
-        mkexpr desc $startpos $endpos }
+        with_location desc $startpos $endpos }
   | constructor = UIDENT arg = simple_expr
       { let desc = Constructor{ constructor; arg } in
-        mkexpr desc $startpos $endpos }
-  | MATCH expr = expr WITH cases = list(case) END
+        with_location desc $startpos $endpos }
+  | MATCH expr = sequence_expr WITH cases = list(case) END
       { let desc = Match{ expr; cases; } in
-        mkexpr desc $startpos $endpos }
+        with_location desc $startpos $endpos }
+  | REF value = simple_expr
+      { let desc = Ref{ value; } in
+        with_location desc $startpos $endpos }
+  | reference = simple_expr COLONEQUALS value = expr
+      { let desc = Set{ reference; value; } in
+        with_location desc $startpos $endpos }
 ;
+
+sequence_expr:
+  | expr = expr
+      { expr }
+  | LET binding = binding params = loption(parameters) EQUALS def = expr IN body = sequence_expr
+      { let desc = Let{ binding; params; def; body; } in
+        with_location desc $startpos $endpos }
+  | FUN params = parameters ARROW body = sequence_expr
+      { let desc = Abs{ params; body } in
+        with_location desc $startpos $endpos }
+  | left = expr SEMI right = sequence_expr
+      { let desc = Sequence{ left; right; } in
+        with_location desc $startpos $endpos }
+;
+
 
 binding:
   | name = LIDENT
@@ -102,7 +135,7 @@ as_binding:
 
 case:
   | BAR constructor = UIDENT arg_binding = binding
-      as_binding = ioption(as_binding) ARROW body = expr
+      as_binding = ioption(as_binding) ARROW body = sequence_expr
         { let location = location $startpos $endpos in
           Destruct { constructor; arg_binding; as_binding; body; location } }
   | BAR binding = binding ARROW body = expr
@@ -110,8 +143,3 @@ case:
           Default { binding; body; location } }
 ;
 
-definition:
-  | LET binding = binding params = loption(parameters) EQUALS def = expr
-      { let location = location $startpos $endpos in
-        { binding; params; def; location } }
-;
