proof/Soundness.v
@@ -9,7 +9,24 @@ Require Import Arith LibLN.
 Require Import Cofinite Definitions Substitution
         Wellformedness Kinding Subtyping Typing.
 
-Hint Constructors value red.
+Hint Constructors red.
+
+(* *************************************************************** *)
+(** * Values do not reduce *)
+
+Lemma values_do_not_reduce : forall t t' V V',
+    value t ->
+    ~ red t V t' V'.
+Proof.
+  introv Hv.
+  unfold not.
+  introv Hr.
+  generalize dependent t'.
+  generalize dependent V.
+  generalize dependent V'.
+  induction Hv; introv Hr;
+    inversion Hr; subst; eauto.
+Qed.
 
 (* *************************************************************** *)
 (** * Preservation *)
@@ -17,44 +34,75 @@ Hint Constructors value red.
 Lemma preservation : preservation.
 Proof.
   unfold preservation.
-  introv Ht Hr.
-  destruct Ht as [Hv [L Ht]].
-  split; auto.
-  exists L; introv Hf.
-  specialize (Ht Xs Hf).
-  remember (instance_vars M Xs) as T.
-  remember (E & Xs ~::* M) as F.
-  clear - Ht Hr.
+  introv Ht Hs Hr.
+  apply validated_typing in Ht.
   generalize dependent T.
-  generalize dependent F.
-  induction Hr; introv Ht.
-  - apply validated_typing in Ht.
+  generalize dependent P.
+  induction Hr; introv Hs Ht.
+  - exists P.
+    splits; auto.
     inversion Ht; subst.
-    pick_fresh x.
-    rewrite trm_subst_intro with (x := x); auto.
-    apply typing_trm_subst_l with (L := L) (M := M); auto.
+    + pick_fresh x.
+      rewrite trm_subst_intro with (x := x); auto with value_regular.
+      apply typing_trm_subst_l with (L := L) (M := M); auto.
+    + pick_fresh x.
+      rewrite trm_subst_intro with (x := x); auto with value_regular.
+      apply typing_trm_subst_empty_l with (T2 := T1); auto.
   - inversion Ht; subst.
-    eauto.
+    + assert (value t1) as Hv by assumption.
+      exfalso.
+      apply (values_do_not_reduce Hv Hr).
+    + assert (typing_validated E P t1 T1) as Ht2 by auto.
+      destruct (IHHr _ Hs _ Ht2) as [P' [He [Ht' Hs']]].
+      exists P'.
+      splits; auto.
+      apply typing_let with (L := L \u dom E) (T1 := T1); auto.
+      eauto 6 using typing_extend_store_type,
+        valid_store_type_add_typ_bind_l, valid_scheme_empty
+        with typing_store_validated.
   - inversion Ht; subst.
-    eauto.
+    assert (typing_validated E P t1 (typ_arrow S T)) as Ht2 by auto.
+    destruct (IHHr _ Hs _ Ht2) as [P' [He [Ht' Hs']]].
+    exists P'.
+    splits; auto.
+    eauto using typing_extend_store_type with typing_store_validated.
   - inversion Ht; subst.
-    eauto.
-  - apply validated_typing in Ht.
+    assert (typing_validated E P t2 S) as Ht2 by auto.
+    destruct (IHHr _ Hs _ Ht2) as [P' [He [Ht' Hs']]].
+    exists P'.
+    splits; auto.
+    eauto using typing_extend_store_type with typing_store_validated.
+  - exists P.
+    splits; auto.
     inversion Ht; subst.
-    assert (typing_validated F (trm_abs t1) (typ_arrow S T)) as Ht2
+    assert (typing_validated E P (trm_abs t1) (typ_arrow S T)) as Ht2
       by assumption.
     inversion Ht2; subst.
     pick_fresh x.
     rewrite trm_subst_intro with (x := x); auto.
     apply typing_trm_subst_empty_l with (T2 := S); auto.
   - inversion Ht; subst.
-    eauto.
+    assert (typing_validated E P t T3) as Ht2 by auto.
+    destruct (IHHr _ Hs _ Ht2) as [P' [He [Ht' Hs']]].
+    exists P'.
+    splits; auto.
+    eauto using typing_extend_store_type with typing_store_validated.
   - inversion Ht; subst.
-    eauto.
-  - apply validated_typing in Ht.
+    assert (typing_validated E P t1 (typ_variant T1)) as Ht2 by auto.
+    destruct (IHHr _ Hs _ Ht2) as [P' [He [Ht' Hs']]].
+    exists P'.
+    splits; auto.
+    apply typing_match with (L := L \u dom E) (T1 := T1) (T2 := T2)
+      (T3 := T3) (T4 := T4) (T5 := T5) (T6 := T6) (T7 := T7); auto;
+      eauto 8 using typing_extend_store_type,
+        valid_store_type_add_typ_bind_l,
+        valid_scheme_empty, kinding_range_top_bot
+        with typing_store_validated.
+  - exists P.
+    splits; auto.
     inversion Ht; subst.
     assert
-      (typing_validated F (trm_constructor c2 t1) (typ_variant T1))
+      (typing_validated E P (trm_constructor c2 t1) (typ_variant T1))
       as Ht2 by assumption.
     inversion Ht2; subst.
     pick_fresh x.
@@ -68,10 +116,11 @@ Proof.
       with (T2 := typ_proj CSet.universe T2 (CSet.singleton c2));
       auto.
     eauto using subtype_proj, subtype_from_ranges with csetdec.
-  - apply validated_typing in Ht.
+  - exists P.
+    splits; auto.
     inversion Ht; subst.
     assert
-      (typing_validated F (trm_constructor c1 t1) (typ_variant T1))
+      (typing_validated E P (trm_constructor c1 t1) (typ_variant T1))
       as Ht2 by assumption.
     inversion Ht2; subst.
     pick_fresh x.
@@ -86,11 +135,20 @@ Proof.
     + eauto using subtype_proj, subtype_from_ranges with csetdec.
     + eauto using subtype_proj_subset with csetdec.
   - inversion Ht; subst.
-    eauto.
-  - apply validated_typing in Ht.
+    assert (typing_validated E P t1 (typ_variant T1)) as Ht2 by auto.
+    destruct (IHHr _ Hs _ Ht2) as [P' [He [Ht' Hs']]].
+    exists P'.
+    splits; auto.
+    apply typing_destruct with (L := L \u dom E)
+      (T1 := T1) (T2 := T2) (T3 := T3); auto.
+    eauto 6 using typing_extend_store_type, 
+      valid_store_type_add_typ_bind_l,
+      valid_scheme_empty with typing_store_validated.
+  - exists P.
+    splits; auto.
     inversion Ht; subst.
     assert
-      (typing_validated F (trm_constructor c2 t1) (typ_variant T1))
+      (typing_validated E P (trm_constructor c2 t1) (typ_variant T1))
       as Ht2 by assumption.
     inversion Ht2; subst.
     pick_fresh x.
@@ -107,7 +165,76 @@ Proof.
       auto.
     eauto using subtype_proj, subtype_from_ranges with csetdec.
   - inversion Ht; subst.
-    eauto.
+    assert (typing_validated E P t (typ_variant T1)) as Ht2 by auto.
+    destruct (IHHr _ Hs _ Ht2) as [P' [He [Ht' Hs']]].
+    exists P'.
+    splits; auto.
+    eauto using typing_extend_store_type with typing_store_validated.
+  - inversion Ht; subst.
+    assert (typing_validated E P t T0) as Ht2 by auto.
+    destruct (IHHr _ Hs _ Ht2) as [P' [He [Ht' Hs']]].
+    exists P'.
+    splits; auto.
+  - inversion Ht; subst.
+    exists (P & l ~ T0).
+    destruct Hs as [_ [_ [? Hv]]].
+    splits; eauto using extends_push.
+    splits; auto.
+    introv Hb.
+    destruct (binds_push_inv Hb) as [[? ?]|[? Hb2]].
+    + subst.
+      exists t.
+      split; auto.
+      eauto 7 using typing_extend_store_type.
+    + destruct (Hv _ _ Hb2) as [t1 [? ?]].
+      exists t1.
+      split; auto.
+      eauto 6 using typing_extend_store_type.
+  - inversion Ht; subst.
+    assert (typing_validated E P t (typ_ref T)) as Ht2 by auto.
+    destruct (IHHr _ Hs _ Ht2) as [P' [He [Ht' Hs']]].
+    exists P'.
+    splits; auto.
+  - exists P.
+    splits; auto.
+    inversion Ht; subst.
+    assert (typing_validated E P (trm_loc l) (typ_ref T)) as Ht2
+        by assumption.
+    inversion Ht2; subst.
+    assert (binds l T1 P) as Hb2 by assumption.
+    destruct Hs as [_ [_ [_ Hv]]].
+    destruct (Hv _ _ Hb2) as [t' [? ?]].
+    replace t with t' by eauto using binds_func.
+    eauto using typing_equal.
+  - inversion Ht; subst.
+    assert (typing_validated E P t1 (typ_ref T0)) as Ht2 by auto.
+    destruct (IHHr _ Hs _ Ht2) as [P' [He [Ht' Hs']]].
+    exists P'.
+    splits; auto.
+    eauto using typing_extend_store_type with typing_store_validated.
+  - inversion Ht; subst.
+    assert (typing_validated E P t2 T0) as Ht2 by auto.
+    destruct (IHHr _ Hs _ Ht2) as [P' [He [Ht' Hs']]].
+    exists P'.
+    splits; auto.
+    eauto using typing_extend_store_type with typing_store_validated.
+  - inversion Ht; subst.
+    exists P.
+    splits; auto.
+    assert (typing_validated E P (trm_loc l) (typ_ref T0)) as Ht2
+        by assumption.
+    inversion Ht2; subst.
+    destruct Hs as [_ [_ [Hn Hv]]].
+    splits; auto.
+    introv Hb.
+    case_if_eq l l0.
+    + exists t2.
+      split; auto.
+      replace T with T1 by eauto using binds_func.
+      eauto using typing_equal, type_equal_symmetric.   
+    + destruct (Hv _ _ Hb) as [t' [? ?]].
+      exists t'.
+      split; auto.
 Qed.
 
 (* *************************************************************** *)
@@ -116,38 +243,41 @@ Qed.
 Lemma progress : progress.
 Proof.
   unfold progress.
-  introv Ht.
-  destruct Ht as [Hv [L Ht]].
-  pick_freshes_gen L (sch_arity M) Xs.
-  specialize (Ht Xs Fr).
-  assert (no_term_bindings (empty & Xs ~::* M)) as Hb
-    by auto with no_term_bindings.
-  remember (empty & Xs ~::* M) as F.
-  remember (instance_vars M Xs) as T.
-  clear - Ht Hb.
+  introv Hb Ht Hv.
   apply validated_typing in Ht.
+  assert (store V) by auto with typing_store_regular.
   induction Ht; auto.
   - exfalso; eapply Hb; eauto.
-  - assert (value t1 \/ (exists t1', red t1 t1')) as IH1 by auto.
-    assert (value t2 \/ (exists t2', red t2 t2')) as IH2 by auto.
-    destruct IH1 as [Hv1|[t1' He1]]; destruct IH2 as [Hv2|[t2' He2]];
-      eauto.
+  - assert (value t1 \/ (exists t1' V1', red t1 V t1' V1'))
+      as IH1 by auto.
+    assert (value t2 \/ (exists t2' V2', red t2 V t2' V2'))
+      as IH2 by auto.
+    destruct IH1 as [Hv1|[t1' [V1' He1]]];
+      destruct IH2 as [Hv2|[t2' [V2' He2]]];
+        eauto.
     destruct Hv1; inversion Ht1; subst; eauto.
   - pick_freshes_gen L (sch_arity M) Xs.
     assert (no_term_bindings (E & Xs ~::* M))
       by auto with no_term_bindings.
-    assert (value t1 \/ (exists t1', red t1 t1')) as IH1 by eauto.
-    destruct IH1 as [Hv1|[t1' He1]]; eauto.
-  - assert (value t \/ (exists t', red t t')) as IH by eauto.
-    destruct IH as [Hv1|[t1' He1]]; eauto.
-  - assert (value t1 \/ (exists t1', red t1 t1')) as IH1 by eauto.
-    destruct IH1 as [Hv1|[t1' He1]]; eauto.
+    assert (value t1 \/ (exists t1' V1', red t1 V t1' V1'))
+      as IH1 by eauto.
+    destruct IH1 as [Hv1|[t1' [V1' He1]]]; eauto 6.
+  - assert (value t1 \/ (exists t1' V1', red t1 V t1' V1'))
+      as IH1 by eauto.
+    destruct IH1 as [Hv1|[t1' [V1' He1]]]; eauto 6.
+  - assert (value t \/ (exists t' V', red t V t' V'))
+      as IH by eauto.
+    destruct IH as [Hv1|[t' [V' He1]]]; eauto 6.
+  - assert (value t1 \/ (exists t1' V1', red t1 V t1' V1'))
+      as IH1 by eauto.
+    destruct IH1 as [Hv1|[t1' [V1' He1]]]; eauto.
     destruct Hv1; inversion Ht; subst.
-    destruct (Nat.eq_dec c c0); subst; eauto.
-  - assert (value t1 \/ (exists t1', red t1 t1')) as IH1 by eauto.
-    destruct IH1 as [Hv1|[t1' He1]]; eauto.
+    destruct (Nat.eq_dec c c0); subst; eauto 6.
+  - assert (value t1 \/ (exists t1' V1', red t1 V t1' V1'))
+      as IH1 by eauto.
+    destruct IH1 as [Hv1|[t1' [V1' He1]]]; eauto.
     destruct Hv1; inversion Ht; subst.
-    destruct (Nat.eq_dec c c0); subst; eauto.
+    destruct (Nat.eq_dec c c0); subst; eauto 6.
     exfalso.
     apply no_subtype_constructor_bot
       with (E := E) (T := T6) (c := c0).
@@ -158,8 +288,9 @@ Proof.
       with (T2 := typ_proj CSet.universe T2 (CSet.singleton c0));
       eauto using subtype_proj, subtype_from_ranges with csetdec.
     eauto using subtype_proj_subset_bottom with csetdec.
-  - assert (value t1 \/ (exists t1', red t1 t1')) as IH1 by eauto.
-    destruct IH1 as [Hv1|[t1' He1]]; eauto.
+  - assert (value t1 \/ (exists t1' V1', red t1 V t1' V1'))
+      as IH1 by eauto.
+    destruct IH1 as [Hv1|[t1' [V1' He1]]]; eauto.
     destruct Hv1; inversion Ht; subst.
     exfalso.
     apply no_subtype_constructor_bot
@@ -173,4 +304,24 @@ Proof.
                 (typ_bot CSet.universe) (CSet.singleton c));
       eauto using subtype_proj, subtype_from_ranges with csetdec.
     auto using subtype_reflexive, type_equal_proj_bot with csetdec.
+  - assert (value t1 \/ (exists t1' V1', red t1 V t1' V1'))
+      as IH1 by eauto.
+    destruct IH1 as [Hv1|[t1' [V1' He1]]]; eauto.
+    pick_fresh_gen (dom V) l; eauto.
+  - assert (value t1 \/ (exists t1' V1', red t1 V t1' V1'))
+      as IH1 by eauto.
+    destruct IH1 as [Hv1|[t1' [V1' He1]]]; eauto.
+    destruct Hv1; inversion Ht; subst.
+    destruct Hv as [_ [_ [_ Hv2]]].
+    assert (binds l T1 P) as Hb2 by assumption.
+    destruct (Hv2 _ _ Hb2) as [t2 [Hb3 _]].
+    eauto.
+  - assert (value t1 \/ (exists t1' V1', red t1 V t1' V1'))
+      as IH1 by eauto.
+    assert (value t2 \/ (exists t2' V2', red t2 V t2' V2'))
+      as IH2 by auto.
+    destruct IH1 as [Hv1|[t1' [V1' He1]]];
+      destruct IH2 as [Hv2|[t2' [V2' He2]]]; eauto.
+    destruct Hv1; inversion Ht1; subst.
+    eauto.
 Qed.
